Prove ILN -> IL correct (required for parsing).

IL/ILN.v
@@ -1,5 +1,5 @@
 Require Import List.
-Require Export Util Var Val Exp Env Map CSet AutoIndTac IL Sim.
+Require Export Util Var Val Exp Env Map CSet AutoIndTac IL Sim Infra.Status.
 
 Set Implicit Arguments.
 
@@ -17,7 +17,7 @@ Inductive nstmt : Type :=
 Fixpoint pos X `{OrderedType X} (l:list X) (x:X) (n:nat) : option nat :=
   match l with 
     | nil => None
-    | y::l => if [ x == y ] then Some n else pos l x (S n)
+    | y::l => if [ x === y ] then Some n else pos l x (S n)
   end.
 
 
@@ -50,9 +50,11 @@ Module F.
     : step (L, E, nstmtIf x b1 b2) (L, E, b2)
 
     
-  | nstepGoto (L:labenv) (E:env val) (l:lab) Y Z (s:nstmt) L' E'
+  | nstepGoto (L:labenv) (E:env val) (l l':lab) Y Z (s:nstmt) L' E'
     (len:length Z = length Y)
-    (Ldef:L (counted l) = Some (blockI L' E' (l,Z,s))) E''
+    (lEQ:l = l') (* hack: otherwise inversions confuse guardedness checker in 
+                  simulation proofs*)
+    (Ldef:L (counted l) = Some (blockI L' E' (l',Z,s))) E''
     (updOk:updE E' E Z Y  = E'')
     : step (L, E, nstmtGoto l Y)
            (L'[(counted l) <- Some (blockI L' E' (l,Z,s))], E'', s)
@@ -98,6 +100,7 @@ Module I.
   
   Definition labenv := env (option block).
   Definition state : Type := (labenv * env val * nstmt)%type.
+  Definition labenv_empty : labenv := fun _ => None.
 
   Inductive step : state -> state -> Prop :=
   | nstepExp L E x e b v
@@ -114,12 +117,13 @@ Module I.
     (condFalse:val2bool (E x) = false)
     : step (L, E, nstmtIf x b1 b2) (L, E, b2)
 
-  | nstepGoto (L:labenv) (E:env val) (l:lab) Y Z (s:nstmt) L'
+  | nstepGoto (L:labenv) (E:env val) (l l':lab) Y Z (s:nstmt) L'
     (len:length Z = length Y)
-    (Ldef:L (counted l) = Some (blockI L' (l,Z,s))) E''
+    (lEQ: l = l')
+    (Ldef:L (counted l) = Some (blockI L' (l',Z,s))) E''
     (updOk:updE E E Z Y  = E'')
     : step (L, E, nstmtGoto l Y)
-           (L'[(counted l) <- Some (blockI L' (l,Z,s))], E'', s)
+           (L'[(counted l) <- Some (blockI L' (l',Z,s))], E'', s)
 
   | stepLet L E f s Z t 
     : step (L, E, nstmtLet f Z s t) (L[counted f <- Some (blockI L (f,Z,s))], E, t).
@@ -150,19 +154,20 @@ Module I.
 
 End I.
 
-Fixpoint labIndices (s:nstmt) (symb: list lab) : option stmt :=
+Fixpoint labIndices (s:nstmt) (symb: list lab) : status stmt :=
   match s with
-    | nstmtExp x e s => mdo s' <- (labIndices s symb); Some (stmtExp x e s')
+    | nstmtExp x e s => sdo s' <- (labIndices s symb); Success (stmtExp x e s')
     | nstmtIf x s1 s2 => 
-      mdo s1' <- (labIndices s1 symb);
-      mdo s2' <- (labIndices s2 symb);
-      Some (stmtIf x s1' s2')
-    | nstmtGoto l Y => mdo f <- pos symb l 0; Some (stmtGoto (LabI f) Y)
-    | nstmtReturn x => Some (stmtReturn x)
+      sdo s1' <- (labIndices s1 symb);
+      sdo s2' <- (labIndices s2 symb);
+      Success (stmtIf x s1' s2')
+    | nstmtGoto l Y => 
+      sdo f <- option2status (pos symb l 0) "labIndices: Undeclared function" ; Success (stmtGoto (LabI f) Y)
+    | nstmtReturn x => Success (stmtReturn x)
     | nstmtLet l Z s1 s2 => 
-      mdo s1' <- labIndices s1 (l::symb);
-      mdo s2' <- labIndices s2 (l::symb);
-      Some (stmtLet Z s1' s2')
+      sdo s1' <- labIndices s1 (l::symb);
+      sdo s2' <- labIndices s2 (l::symb);
+      Success (stmtLet Z s1' s2')
   end.
 
 Definition state_result X (s:X*env val*nstmt) : option val :=
@@ -190,38 +195,165 @@ Tactic Notation "goto_invs" tactic(tac) :=
         | no_step; tac; simpl in *; eauto ]
   end.
 
+Inductive lab_approx : list lab -> env (option I.block) -> list IL.I.block -> Prop :=
+  Lai symb L L'
+    (LEQ: forall f f' s Z Lb, 
+             L (counted f) = Some (I.blockI Lb (f',Z,s)) 
+             -> exists i s',   
+                 get L' i (IL.I.blockI Z s')
+                 /\ labIndices s (drop i symb) = Success s'
+                 /\ pos symb f 0 = Some i                                                             /\ lab_approx (drop (S i) symb) (Lb (* [counted f <- Some (I.blockI Lb (f, Z, s))] *)) (drop (S i) L')
+                 /\ (forall l b, Lb (counted l) = Some b -> fst (fst (I.block_F b)) = l)
+                 /\ (forall f i' k, pos (drop (S i) symb) f k = Some i' -> Lb (counted f) <> None) 
+                 /\ f = f') 
+  : lab_approx symb L L'.
+
 Inductive labIndicesSim : I.state -> IL.I.state -> Prop :=
   | labIndicesSimI (L:env (option I.block)) L' E s s' symb
-    (EQ:labIndices s symb = Some s')
-    (LEQ: forall f Lb Z s, L (counted f) = Some (I.blockI Lb (f,Z,s))
-                 -> exists i s', pos symb f 0 = Some i /\ get L' i (IL.I.blockI Z s'))
+    (EQ:labIndices s symb = Success s')
+    (LA:lab_approx symb L L')
+    (LL:forall l b, L (counted l) = Some b -> fst (fst (I.block_F b)) = l)
+    (EX:forall f i k, pos symb f k = Some i -> L (counted f) <> None)
   : labIndicesSim (L, E, s) (L', E, s').
+
+
+Lemma modus_ponens P Q
+: P -> (P -> Q) -> Q.
+tauto.
+Qed.
+
+Tactic Notation "exploiT" tactic(tac) :=
+  eapply modus_ponens;[ tac | intros].
+
+Ltac exploit H :=
+  eapply modus_ponens;[ eapply H | intros].
+
+      
+Lemma pos_add k' symb (f:lab) k i
+: pos symb f k = Some i -> pos symb f (k' + k) = Some (k' + i).
+Proof.
+  general induction symb; eauto.
+  unfold pos in *; fold pos in *.
+  destruct if. congruence.
+  eapply IHsymb in H. orewrite (S (k' + k) = k' + S k). eauto.
+Qed.
+
+Lemma pos_sub k' symb (f:lab) k i
+: pos symb f (k' + k) = Some (k' + i) -> pos symb f k = Some i.
+Proof.
+  general induction symb; eauto.
+  unfold pos in *; fold pos in *.
+  destruct if. f_equal. inv H. omega.
+  orewrite (S (k' + k) = k' + S k) in H. 
+  eauto.
+Qed.
+
+Lemma pos_ge symb (l:lab) i k
+: pos symb l k = Some i
+  -> k <= i.
+Proof.
+  general induction symb. unfold pos in H; fold pos in H.
+  destruct if in H. inv H. cbv in e. omega.
+  exploit IHsymb; eauto. omega.
+Qed.
+
+Lemma pos_drop_eq symb (l:lab) x
+: pos symb l 0 = Some x
+          -> drop x symb = l::tl (drop x symb).
+Proof.
+  general induction symb. 
+  unfold pos in H; fold pos in H. destruct if in H.
+  inv H; inv e; eauto.
+  destruct x. exfalso. exploit pos_ge; eauto. omega.
+  simpl. erewrite IHsymb; eauto. 
+  eapply (pos_sub 1); eauto.
+Qed.
+
+Lemma pos_plus symb (f:lab) n i
+: pos symb f 0 = Some (n + i)
+  -> pos (drop n symb) f 0 = Some i.
+Proof.
+  general induction n; simpl; eauto.
+  destruct symb; simpl.
+  + inv H.
+  + eapply IHn; eauto. simpl in H; destruct if in H. 
+    * inv H. 
+    * eapply (pos_sub 1); eauto.
+Qed.
 
 Lemma labIndicesSim_sim σ1 σ2
   : labIndicesSim σ1 σ2 -> sim σ1 σ2.
 Proof.
   revert σ1 σ2. cofix; intros.
-  destruct H; destruct s; simpl in *; try monad_inv EQ.
+  destruct H; destruct s; simpl in *; try monadS_inv EQ.
   - case_eq (exp_eval E e); intros. 
     + one_step. eapply labIndicesSim_sim; econstructor; eauto.
     + no_step.
-  - case_eq (val2bool (E x)); intros; one_step; eapply labIndicesSim_sim; econstructor; eauto.
+  - case_eq (val2bool (E x)); intros; one_step; eapply labIndicesSim_sim; econstructor; eauto. 
   - case_eq (L (counted l)); intros.
-    + destruct b as [? [[? ?] ?]].
-      destruct_prop (l = l0); subst.
-      edestruct LEQ as [? [? []]]; eauto.
-      assert (x = x0) by congruence; subst.
-      eapply simS. eapply plusO. econstructor; try eapply H; try reflexivity.
-      admit. 
-      eapply plusO. constructor; eauto. simpl. admit.
-      admit.
-      admit.
-    + no_step. admit.
+    + destruct b as [? [[l0 Z'] s']].
+      eapply option2status_inv in EQ0.
+      inv LA.
+      edestruct LEQ as [? [? ?]]; dcr; eauto.
+      assert (x0 = x) by congruence; subst x0.
+      destruct_prop (length Z' = length Y).
+      eapply simS; try eapply plusO.
+      econstructor. try eapply H1; eauto; try reflexivity.
+      symmetry. eapply LL; eauto. eapply H. reflexivity.
+      econstructor; eauto. simpl. eauto.
+      eapply labIndicesSim_sim.
+      econstructor; eauto. subst l0.
+      * simpl.
+        econstructor. simpl; intros; dcr.
+        lud. inv H0.         
+        assert (f = f') by (destruct f, f'; simpl in *; congruence); subst.
+        do 2 eexists. split.
+        eapply drop_get with (n:=0). orewrite (x + 0 = x). eauto.
+        intuition. 
+        eapply pos_plus. orewrite (x + 0 = x); eauto.
+        simpl in *. repeat rewrite drop_tl. auto.
+        eapply H6. simpl in H8. rewrite drop_tl in H8. eapply H8. eauto.
+        inv H4.
+        edestruct (LEQ0); eauto. destruct H9; dcr.
+        eexists (S x0), x2. split; eauto using get. 
+        eapply drop_get. orewrite (x + S x0 = S x + x0). eapply get_drop. eauto.
+        repeat rewrite drop_tl in *. repeat rewrite drop_drop in *.
+        orewrite (S x0 + x = x0 + S x); eauto.
+        repeat (split; eauto). 
+        exploit pos_drop_eq; [eapply H2|].
+        rewrite X. unfold pos; fold pos. destruct if. congruence.
+        rewrite drop_tl. eapply (pos_add 1); eauto.       
+      * subst l0. intros. lud. inv H0.
+        assert (l = l0) by (destruct l, l0; simpl in *; congruence); subst.                 simpl; eauto.
+        eapply H5; eauto.
+      * subst l. intros. lud. congruence. eapply H6; eauto. 
+        exploit pos_drop_eq; [eapply H2|].
+        rewrite X in H0. unfold pos in H0; fold pos in H0.
+        destruct if in H0. congruence.
+        simpl. rewrite <- drop_tl. eauto.
+      * subst l. no_step. simpl in *. (*rewrite H in Ldef. inv Ldef. congruence. *)
+        simpl in *. get_functional; subst. simpl in *. congruence.
+    + eapply option2status_inv in EQ0. exfalso. eapply EX; eauto.
   - no_step.
   - one_step. eapply labIndicesSim_sim. econstructor; eauto.
-    admit.
-Admitted.
-
+    econstructor. intros. 
+    + lud. 
+      * inv H. do 2 eexists.
+        split. econstructor. intuition. unfold pos; fold pos.
+        destruct if; eauto. cbv in n; destruct f, f'; simpl in *; congruence.
+        destruct f, f'; simpl in *; congruence.
+      * inv LA. edestruct LEQ; eauto. destruct H2.
+        eexists (S x1),x2. dcr. split; eauto using get.
+        split; eauto. split; eauto.
+        unfold pos; fold pos. destruct if; eauto.
+                                         congruence.
+        intros. eapply (pos_add 1); eauto. 
+    + intros. lud; eauto. 
+      inv H; eauto. destruct l, l0; simpl in *; congruence; eauto.
+    + intros. lud. congruence. 
+      unfold pos in H; fold pos in H. 
+      destruct if in H. congruence. eapply EX; eauto.
+Qed.
 
 (* 
 *** Local Variables: ***
